Set up wal recovery theorems

src/program_proof/wal/invariant.v
@@ -524,6 +524,26 @@ Definition is_wal_inner_durable γ s dinit : iProp Σ :=
                     "Hcirc" ∷ is_circular_state γ.(circ_name) cs
 .
 
+Definition wal_init_ghost_state (γnew: wal_names) : iProp Σ :=
+    ghost_var γnew.(installer_pos_name) 1 (U64 0) ∗
+    ghost_var γnew.(installer_txn_id_name) 1 0%nat ∗
+    ghost_var γnew.(diskEnd_mem_name) 1 0%nat ∗
+    ghost_var γnew.(diskEnd_mem_txn_id_name) 1 0%nat.
+
+Definition is_wal_inner_crash (γold: wal_names) s' : iProp Σ := True.
+
+Definition wal_ghost_exchange (γold γnew: wal_names) : iProp Σ := True.
+
+Lemma wal_crash_upd l γold γnew s s' dinit :
+  relation.denote log_crash s s' () →
+  is_wal_inner l γold s dinit -∗ wal_init_ghost_state γnew ==∗
+  is_wal_inner_durable γnew s' dinit ∗
+  is_wal_inner_crash γold s' ∗
+  wal_ghost_exchange γold γnew.
+Proof.
+  (* TODO: start this proof *)
+Admitted.
+
 (* This is produced by recovery as a post condition, can be used to get is_wal *)
 Definition is_wal_inv_pre (l: loc) γ s (dinit : disk) : iProp Σ :=
   is_wal_inner l γ s dinit ∗ (∃ cs, is_circular_state γ.(circ_name) cs ∗ circular_pred γ cs).
